shift-reset/core/syntax_notation.v
@@ -8,7 +8,8 @@ Local Open Scope term_scope.
 Declare Custom Entry binder'.
 Declare Custom Entry pattern'.
 Declare Custom Entry term.
-Declare Custom Entry abs_term.
+Declare Custom Entry term1.
+Declare Custom Entry term2.
 Declare Custom Entry ret_term.
 Declare Custom Entry exn_term.
 Declare Custom Entry eff_term.
@@ -20,14 +21,14 @@ Notation "'_'" := PAny (in custom pattern' at level 0) : term_scope.
 Notation "x" := x (in custom pattern' at level 0, x constr at level 0) : term_scope.
 
 Notation "' ( tag x )" :=
-  (PConstr tag x) (in custom pattern' at level 10, tag at level 0, x custom binder') : term_scope.
+  (PConstr tag x) (in custom pattern' at level 10, tag at level 0, x custom binder' at level 0) : term_scope.
 
-Notation "' ( tag x 'as' y )" :=
-  (PAlias (PConstr tag x) y)
+Notation "' ( tag x1 'as' x2 )" :=
+  (PAlias (PConstr tag x1) x2)
     (in custom pattern' at level 10,
         tag at level 0,
-        x custom binder',
-        y constr at level 0) : term_scope.
+        x1 custom binder' at level 0,
+        x2 constr at level 0) : term_scope.
 
 Notation "<{ t }>" := t (t custom term at level 99) : term_scope.
 Notation "( t )" := t (in custom term, t at level 99) : term_scope.
@@ -35,7 +36,14 @@ Notation "{ t }" := t (in custom term, t constr) : term_scope.
 Notation "t" := t (in custom term at level 0, t constr at level 0) : term_scope.
 
 Notation "( 'fun' x => t )" :=
-  (TAbs x t) (in custom abs_term at level 69, x custom binder' at level 0, t custom term) : term_scope.
+  (T1 x t) (in custom term1 at level 69, x custom binder' at level 0, t custom term) : term_scope.
+
+Notation "( 'fun' x1 x2 => t )" :=
+  (T2 x1 x2 t)
+    (in custom term2 at level 69,
+        x1 custom binder' at level 0,
+        x2 custom binder' at level 0,
+        t custom term) : term_scope.
 
 Notation "( 'fun' x => t )" :=
   (TRetSome x t) (in custom ret_term at level 69, x custom binder' at level 0, t custom term) : term_scope.
@@ -78,7 +86,7 @@ Notation "'if' t1 'then' t2 'else' t3" :=
         t3 custom term) : term_scope.
 
 Notation "'let' x := t1 'in' t2" :=
-  (TLet t1 (TAbs x t2))
+  (TLet t1 (T1 x t2))
     (in custom term at level 69,
         x custom binder' at level 0,
         t1 custom term,
@@ -93,7 +101,7 @@ Notation "t1 ; t2" :=
         right associativity) : term_scope.
 
 Notation "'let' f x1 .. xn := t1 'in' t2" :=
-  (TLet (TVFun (TAbs x1 .. (TVFun (TAbs xn t1)) ..)) (TAbs f t2))
+  (TLet (TVFun (T1 x1 .. (TVFun (T1 xn t1)) ..)) (T1 f t2))
     (in custom term at level 69,
         f custom binder' at level 0,
         x1 custom binder' at level 0,
@@ -103,7 +111,7 @@ Notation "'let' f x1 .. xn := t1 'in' t2" :=
         right associativity) : term_scope.
 
 Notation "'let' 'fix' f x := t1 'in' t2" :=
-  (TLet (TVFix (TAbs2 f x t1)) (TAbs f t2))
+  (TLet (TVFix (T2 f x t1)) (T1 f t2))
     (in custom term at level 69,
         f custom binder' at level 0,
         x custom binder' at level 0,
@@ -112,7 +120,7 @@ Notation "'let' 'fix' f x := t1 'in' t2" :=
         right associativity) : term_scope.
 
 Notation "'let' 'fix' f x1 x2 .. xn := t1 'in' t2" :=
-  (TLet (TVFix (TAbs2 f x1 (TVFun (TAbs x2 .. (TVFun (TAbs xn t1)) ..)))) (TAbs f t2))
+  (TLet (TVFix (T2 f x1 (TVFun (T1 x2 .. (TVFun (T1 xn t1)) ..)))) (T1 f t2))
     (in custom term at level 69,
         f custom binder' at level 0,
         x1 custom binder' at level 0,
@@ -123,16 +131,16 @@ Notation "'let' 'fix' f x1 x2 .. xn := t1 'in' t2" :=
         right associativity) : term_scope.
 
 Notation "'shift' t" :=
-  (TShift tag_empty t) (in custom term at level 69, t custom abs_term) : term_scope.
+  (TShift tag_empty t) (in custom term at level 69, t custom term1) : term_scope.
 
 Notation "'shift' 'at' tag t" :=
-  (TShift tag t) (in custom term at level 69, tag at level 0, t custom abs_term) : term_scope.
+  (TShift tag t) (in custom term at level 69, tag at level 0, t custom term1) : term_scope.
 
 Notation "'control' t" :=
-  (TControl tag_empty t) (in custom term at level 69, t custom abs_term) : term_scope.
+  (TControl tag_empty t) (in custom term at level 69, t custom term1) : term_scope.
 
 Notation "'control' 'at' tag t" :=
-  (TControl tag t) (in custom term at level 69, tag at level 0, t custom abs_term) : term_scope.
+  (TControl tag t) (in custom term at level 69, tag at level 0, t custom term1) : term_scope.
 
 Notation "'reset' t" :=
   (TReset tag_empty t) (in custom term at level 69, t custom term) : term_scope.
@@ -147,21 +155,21 @@ Notation "'prompt' 'at' tag t" :=
   (TPrompt tag t) (in custom term at level 69, tag at level 0, t custom term) : term_scope.
 
 Notation "'fun' x1 .. xn => t" :=
-  (TVFun (TAbs x1 .. (TVFun (TAbs xn t)) ..))
+  (TVFun (T1 x1 .. (TVFun (T1 xn t)) ..))
     (in custom term at level 69,
         x1 custom binder' at level 0,
         xn custom binder' at level 0,
         t custom term at level 99) : term_scope.
 
 Notation "'fix' f x := t" :=
-  (TVFix (TAbs2 f x t))
+  (TVFix (T2 f x t))
     (in custom term at level 69,
         f custom binder' at level 0,
         x custom binder' at level 0,
         t custom term at level 99) : term_scope.
 
 Notation "'fix' f x1 x2 .. xn := t" :=
-  (TVFix (TAbs2 f x1 (TVFun (TAbs x2 .. (TVFun (TAbs xn t)) ..))))
+  (TVFix (T2 f x1 (TVFun (T1 x2 .. (TVFun (T1 xn t)) ..))))
     (in custom term at level 69,
         f custom binder' at level 0,
         x1 custom binder' at level 0,
@@ -173,11 +181,14 @@ Notation "()" := TVUnit (in custom term at level 0) : term_scope.
 Notation "'true'" := TVTrue (in custom term at level 0) : term_scope.
 Notation "'false'" := TVFalse (in custom term at level 0) : term_scope.
 
-Notation "'not' t" :=
-  (TVNot t) (in custom term at level 23, t custom term at level 0) : term_scope.
+Notation "+ t" :=
+  (Op1Pos t) (in custom term at level 23, t custom term at level 0) : term_scope.
 
 Notation "- t" :=
-  (TVNeg t) (in custom term at level 23, t custom term at level 0) : term_scope.
+  (Op1Neg t) (in custom term at level 23, t custom term at level 0) : term_scope.
+
+Notation "'not' t" :=
+  (Op1Not t) (in custom term at level 23, t custom term at level 0) : term_scope.
 
 Notation "'ref' t" :=
   (TVRef t) (in custom term at level 23, t custom term at level 0) : term_scope.
@@ -192,37 +203,37 @@ Notation "'assert' t" :=
   (TVAssert t) (in custom term at level 23, t custom term at level 0) : term_scope.
 
 Notation "t1 + t2" :=
-  (TVAdd t1 t2) (in custom term at level 40, t1 custom term, t2 custom term) : term_scope.
+  (Op2Add t1 t2) (in custom term at level 40, t1 custom term, t2 custom term) : term_scope.
 
 Notation "t1 - t2" :=
-  (TVSub t1 t2) (in custom term at level 40, t1 custom term, t2 custom term) : term_scope.
+  (Op2Sub t1 t2) (in custom term at level 40, t1 custom term, t2 custom term) : term_scope.
 
 Notation "t1 * t2" :=
-  (TVMul t1 t2) (in custom term at level 39, t1 custom term, t2 custom term) : term_scope.
+  (Op2Mul t1 t2) (in custom term at level 39, t1 custom term, t2 custom term) : term_scope.
 
 Notation "t1 / t2" :=
-  (TVDiv t1 t2) (in custom term at level 39, t1 custom term, t2 custom term) : term_scope.
+  (Op2Div t1 t2) (in custom term at level 39, t1 custom term, t2 custom term) : term_scope.
 
 Notation "t1 'mod' t2" :=
-  (TVMod t1 t2) (in custom term at level 39, t1 custom term, t2 custom term) : term_scope.
+  (Op2Mod t1 t2) (in custom term at level 39, t1 custom term, t2 custom term) : term_scope.
 
 Notation "t1 = t2" :=
-  (TVEq t1 t2) (in custom term at level 50, t1 custom term, t2 custom term) : term_scope.
-
-Notation "t1 <= t2" :=
-  (TVLe t1 t2) (in custom term at level 50, t1 custom term, t2 custom term) : term_scope.
-
-Notation "t1 > t2" :=
-  (TVGt t1 t2) (in custom term at level 50, t1 custom term, t2 custom term) : term_scope.
-
-Notation "t1 >= t2" :=
-  (TVGe t1 t2) (in custom term at level 50, t1 custom term, t2 custom term) : term_scope.
-
-Notation "t1 <> t2" :=
-  (TVNeq t1 t2) (in custom term at level 50, t1 custom term, t2 custom term) : term_scope.
+  (Op2Eqb t1 t2) (in custom term at level 50, t1 custom term, t2 custom term) : term_scope.
 
 Notation "t1 < t2" :=
-  (TVLt t1 t2) (in custom term at level 50, t1 custom term, t2 custom term) : term_scope.
+  (Op2Ltb t1 t2) (in custom term at level 50, t1 custom term, t2 custom term) : term_scope.
+
+Notation "t1 <= t2" :=
+  (Op2Leb t1 t2) (in custom term at level 50, t1 custom term, t2 custom term) : term_scope.
+
+Notation "t1 > t2" :=
+  (Op2Gtb t1 t2) (in custom term at level 50, t1 custom term, t2 custom term) : term_scope.
+
+Notation "t1 >= t2" :=
+  (Op2Geb t1 t2) (in custom term at level 50, t1 custom term, t2 custom term) : term_scope.
+
+Notation "t1 <> t2" :=
+  (Op2Neqb t1 t2) (in custom term at level 50, t1 custom term, t2 custom term) : term_scope.
 
 Notation "t1 && t2" :=
   (TVAnd t1 t2) (in custom term at level 50, t1 custom term, t2 custom term, right associativity) : term_scope.
@@ -237,7 +248,7 @@ Notation "t1 , t2" :=
   (TVPair t1 t2) (in custom term at level 65, t1 custom term, t2 custom term) : term_scope.
 
 Notation "'let' ( x1 , x2 ) := t1 'in' t2" :=
-  (TSplit t1 (TAbs2 x1 x2 t2))
+  (TSplit t1 (T2 x1 x2 t2))
     (in custom term at level 69,
         x1 custom binder' at level 0,
         x2 custom binder' at level 0,
@@ -246,7 +257,7 @@ Notation "'let' ( x1 , x2 ) := t1 'in' t2" :=
         right associativity) : term_scope.
 
 Notation "'let' x1 , x2 := t1 'in' t2" :=
-  (TSplit t1 (TAbs2 x1 x2 t2))
+  (TSplit t1 (T2 x1 x2 t2))
     (in custom term at level 69,
         x1 custom binder' at level 0,
         x2 custom binder' at level 0,
@@ -261,7 +272,7 @@ Notation "'Inr' t" :=
   (TVInr t) (in custom term at level 23, t custom term at level 0) : term_scope.
 
 Notation "'match' tv 'with' | 'Inl' x1 => t1 | 'Inr' x2 => t2 'end'" :=
-  (TCase tv (TAbs x1 t1) (TAbs x2 t2))
+  (TCase tv (T1 x1 t1) (T1 x2 t2))
     (in custom term at level 69,
         tv custom term,
         x1 custom binder' at level 0,
