shift-reset/interpreter/imonad.v
@@ -9,13 +9,13 @@ Arguments imonad_run {A} _ _ _.
 Definition imonad_ask_env : imonad env :=
   IMonad (fun env h => (inr env, h)).
 
-Definition imonad_local_env {A} (f : env -> env) (m : imonad A) : imonad A :=
-  IMonad (fun env => imonad_run m (f env)).
-
 Definition imonad_asks_env {A} (f : env -> A) : imonad A :=
   IMonad (fun env h => (inr (f env), h)).
 
-Definition imonad_use_env {A} (env : env) (m : imonad A) : imonad A :=
+Definition imonad_local_env {A} (f : env -> env) (m : imonad A) : imonad A :=
+  IMonad (fun env => imonad_run m (f env)).
+
+Definition imonad_under_env {A} (env : env) (m : imonad A) : imonad A :=
   IMonad (fun _ => imonad_run m env).
 
 Definition imonad_get_heap : imonad iheap :=
@@ -96,7 +96,7 @@ Definition imonad_replace {A B} (x : A) (m : imonad B) : imonad A :=
 Definition imonad_pure {A} (x : A) : imonad A :=
   IMonad (fun _ h => (inr x, h)).
 
-Definition imonad_ap {A B} (m1 : imonad (A -> B)) (m2 : imonad A) : imonad B :=
+Definition imonad_app {A B} (m1 : imonad (A -> B)) (m2 : imonad A) : imonad B :=
   IMonad (fun env h =>
             let (r, h) := imonad_run m1 env h in
             match r with
@@ -159,7 +159,7 @@ Bind Scope imonad_scope with imonad.
 
 Notation "f <$> m" := (imonad_map f m) (at level 65, right associativity) : imonad_scope.
 Notation "x <$ m" := (imonad_replace x m) (at level 65, right associativity) : imonad_scope.
-Notation "m1 <*> m2" := (imonad_ap m1 m2) (at level 55, left associativity) : imonad_scope.
+Notation "m1 <*> m2" := (imonad_app m1 m2) (at level 55, left associativity) : imonad_scope.
 Notation "m >>= f" := (imonad_bind m f) (at level 50, left associativity) : imonad_scope.
 Notation "m1 >> m2" := (imonad_then m1 m2) (at level 50, left associativity) : imonad_scope.
 Notation "f1 >=> f2" := (imonad_kleisli_compose f1 f2) (at level 60, right associativity) : imonad_scope.
