shift-reset/interpreter/interpreter.v
@@ -1,8 +1,7 @@
 From Stdlib Require Import String Qcanon ZArith.
-From shift_reset.core Require Import syntax env kont loc tag val var.
+From shift_reset.core Require Import syntax env loc tag val var.
 From shift_reset.interpreter Require Import dispatch ierror iheap imonad unwrap.
 
-Local Open Scope list_scope.
 Local Open Scope string_scope.
 Local Open Scope imonad_scope.
 Local Unset Elimination Schemes.
@@ -18,15 +17,8 @@ Fixpoint interpret_val_term (t : val_term) : imonad val :=
   | TVUnit => imonad_pure VUnit
   | TVInt z => imonad_pure (VInt z)
   | TVFloat q => imonad_pure (VFloat q)
-  | TVNeg t' => interpret_val_term t' >>= dispatch_neg
-  | TVAdd t1 t2 => v <- interpret_val_term t1; f <- dispatch_add v; interpret_val_term t2 >>= f
-  | TVSub t1 t2 => v <- interpret_val_term t1; f <- dispatch_sub v; interpret_val_term t2 >>= f
-  | TVMul t1 t2 => v <- interpret_val_term t1; f <- dispatch_mul v; interpret_val_term t2 >>= f
-  | TVDiv t1 t2 => v <- interpret_val_term t1; f <- dispatch_div v; interpret_val_term t2 >>= f
-  | TVMod t1 t2 => v <- interpret_val_term t1; f <- dispatch_mod v; interpret_val_term t2 >>= f
   | TVTrue => imonad_pure VTrue
   | TVFalse => imonad_pure VFalse
-  | TVNot t' => interpret_val_term t' >>= dispatch_not
   | TVAnd t1 t2 =>
       v <- interpret_val_term t1;
       b <- unwrap_vbool v;
@@ -37,7 +29,9 @@ Fixpoint interpret_val_term (t : val_term) : imonad val :=
       if b then imonad_pure VTrue else interpret_val_term t2
   | TVFun t' => imonad_asks_env (VFun' t')
   | TVFix t' => imonad_asks_env (VFix' t')
-  | TVPair t1 t2 => v <- interpret_val_term t1; VPair v <$> interpret_val_term t2
+  | TVPair t1 t2 =>
+      v <- interpret_val_term t1;
+      VPair v <$> interpret_val_term t2
   | TVInl t' => VInl <$> interpret_val_term t'
   | TVInr t' => VInr <$> interpret_val_term t'
   | TVRef t' =>
@@ -78,240 +72,220 @@ Fixpoint interpret_val_term (t : val_term) : imonad val :=
       v <- interpret_val_term t';
       b <- unwrap_vbool v;
       if b then imonad_pure VUnit else imonad_throw_error (Assert_failure "")
-  | TVLt t1 t2 => v <- interpret_val_term t1; f <- dispatch_lt v; interpret_val_term t2 >>= f
-  | TVLe t1 t2 => v <- interpret_val_term t1; f <- dispatch_le v; interpret_val_term t2 >>= f
-  | TVGt t1 t2 => v <- interpret_val_term t1; f <- dispatch_gt v; interpret_val_term t2 >>= f
-  | TVGe t1 t2 => v <- interpret_val_term t1; f <- dispatch_ge v; interpret_val_term t2 >>= f
-  | TVEq t1 t2 => v <- interpret_val_term t1; f <- dispatch_eq v; interpret_val_term t2 >>= f
-  | TVNeq t1 t2 => v <- interpret_val_term t1; f <- dispatch_neq v; interpret_val_term t2 >>= f
+  | TVOp1 op t' => interpret_val_term t' >>= dispatch_op1 op
+  | TVOp2 op t1 t2 =>
+      v <- interpret_val_term t1;
+      f <- dispatch_op2 op v;
+      interpret_val_term t2 >>= f
+  end.
+
+Definition with_binder (b : binder) (v : val) (env : env) : syntax.env :=
+  match b with
+  | BAny => env
+  | BVar x => EnvCons x v env
+  end.
+
+Fixpoint match_exn (p : pattern) (exn : exn) (env : env) : option syntax.env :=
+  match p with
+  | PAny => Some env
+  | PVar x => Some (EnvCons x (VExn exn) env)
+  | PConstr tag b =>
+      let (tag', v) := exn in
+      if tag_eqb tag tag' then Some (with_binder b v env) else None
+  | PAlias p' x =>
+      match match_exn p' exn env with
+      | Some env' => Some (EnvCons x (VExn exn) env')
+      | None => None
+      end
+  end.
+
+Fixpoint match_eff (p : pattern) (b : binder) (eff : eff) (v : val) (env : env) : option syntax.env :=
+  match p with
+  | PAny => Some (with_binder b v env)
+  | PVar x => Some (EnvCons x (VEff eff) (with_binder b v env))
+  | PConstr tag b' =>
+      let (tag', v') := eff in
+      if tag_eqb tag tag' then Some (with_binder b' v' (with_binder b v env)) else None
+  | PAlias p' x =>
+      match match_eff p' b eff v env with
+      | Some env' => Some (EnvCons x (VEff eff) env')
+      | None => None
+      end
   end.
 
 Inductive iresult : Type :=
-| RVal : val -> iresult
-| RShift : metakont -> (val -> imonad iresult) -> tag -> iresult
-| RControl : metakont -> (val -> imonad iresult) -> tag -> iresult
-| RRaise : exn -> iresult
-| RPerform : metakont -> eff -> iresult.
+| IRVal : val -> iresult
+| IRShift : metakont -> (val -> imonad iresult) -> tag -> iresult
+| IRControl : metakont -> (val -> imonad iresult) -> tag -> iresult
+| IRRaise : exn -> iresult
+| IRPerform : metakont -> eff -> iresult.
 
-Definition with_binder (b : binder) (v : val) (m : imonad iresult) : imonad iresult :=
-  match b with
-  | BAny => m
-  | BVar x => imonad_local_env (EnvCons x v) m
-  end.
+Record ikont : Type := IKont { ikont_car :> kont; ikont_app :> val -> imonad iresult }.
 
-Definition with_binder2 (b1 b2 : binder) (v1 v2 : val) (m : imonad iresult) : imonad iresult :=
-  with_binder b2 v2 (with_binder b1 v1 m).
+Definition ikont_nil : ikont := IKont KNil (fun v => imonad_pure (IRVal v)).
 
-Fixpoint match_exn (p : pattern) (exn : exn) : option (imonad iresult -> imonad iresult) :=
-  match p with
-  | PAny => Some (fun m => m)
-  | PVar x => Some (imonad_local_env (EnvCons x (VExn exn)))
-  | PConstr tag b =>
-      let (tag', v) := exn in
-      if tag_eqb tag tag' then Some (with_binder b v) else None
-  | PAlias p' x =>
-      match match_exn p' exn with
-      | Some f => Some (fun m => imonad_local_env (EnvCons x (VExn exn)) (f m))
-      | None => None
-      end
-  end.
-
-Fixpoint match_eff (p : pattern) (b : binder) (eff : eff) (v : val) : option (imonad iresult -> imonad iresult) :=
-  match p with
-  | PAny => Some (with_binder b v)
-  | PVar x => Some (fun m => imonad_local_env (EnvCons x (VEff eff)) (with_binder b v m))
-  | PConstr tag b' =>
-      let (tag', v') := eff in
-      if tag_eqb tag tag' then Some (with_binder2 b b' v v') else None
-  | PAlias p' x =>
-      match match_eff p' b eff v with
-      | Some f => Some (fun m => imonad_local_env (EnvCons x (VEff eff)) (f m))
-      | None => None
-      end
-  end.
-
-Record ikont : Type := IKont { ikont_head : kont; ikont_tail : list kont; ikont_app :> val -> imonad iresult }.
-
-Fixpoint ikont_car_aux (k : kont) (ks : list kont) : kont :=
-  match ks with
-  | nil => k
-  | k' :: ks' => kont_append k (ikont_car_aux k' ks')
-  end.
-
-Definition ikont_car (k : ikont) : kont :=
-  let (h, t, _) := k in ikont_car_aux h t.
-
-Local Coercion ikont_car : ikont >-> kont.
-
-Definition interpreter : Type := ikont -> term -> imonad iresult.
+Definition interpreter : Type := term -> ikont -> imonad iresult.
 
 Fixpoint unwind_reset (tag : tag) (k : ikont) (r : iresult) : imonad iresult :=
   match r with
-  | RVal v => k v
-  | RShift mk f tag' =>
+  | IRVal v => k v
+  | IRShift mk f tag' =>
       if tag_eqb tag tag'
       then f (VMKReset mk tag) >>= unwind_reset tag k
-      else imonad_pure (RShift (MKReset mk tag k) f tag')
-  | RControl mk f tag' => imonad_pure (RControl (MKReset mk tag k) f tag')
-  | RRaise _ => imonad_pure r
-  | RPerform mk eff => imonad_pure (RPerform (MKReset mk tag k) eff)
+      else imonad_pure (IRShift (MKReset mk tag k) f tag')
+  | IRControl mk f tag' => imonad_pure (IRControl (MKReset mk tag k) f tag')
+  | IRRaise _ => imonad_pure r
+  | IRPerform mk eff => imonad_pure (IRPerform (MKReset mk tag k) eff)
   end.
 
 Fixpoint unwind_prompt (tag : tag) (k : ikont) (r : iresult) : imonad iresult :=
   match r with
-  | RVal v => k v
-  | RShift mk f tag' => imonad_pure (RShift (MKPrompt mk tag k) f tag')
-  | RControl mk f tag' =>
+  | IRVal v => k v
+  | IRShift mk f tag' => imonad_pure (IRShift (MKPrompt mk tag k) f tag')
+  | IRControl mk f tag' =>
       if tag_eqb tag tag'
       then f (VMKPure mk) >>= unwind_prompt tag k
-      else imonad_pure (RControl (MKPrompt mk tag k) f tag')
-  | RRaise _ => imonad_pure r
-  | RPerform mk eff => imonad_pure (RPerform (MKPrompt mk tag k) eff)
+      else imonad_pure (IRControl (MKPrompt mk tag k) f tag')
+  | IRRaise _ => imonad_pure r
+  | IRPerform mk eff => imonad_pure (IRPerform (MKPrompt mk tag k) eff)
   end.
 
-Definition interpret_abs_term_with (self : interpreter) (k : ikont) (t : abs_term) (v : val) : imonad iresult :=
-  let (b, t') := t in with_binder b v (self k t').
+Definition interpret_term1_aux (self : interpreter) (t : term1) (k : ikont) (v : val) : imonad iresult :=
+  let (b, t') := t in imonad_local_env (with_binder b v) (self t' k).
 
-Definition interpret_abs2_term_with (self : interpreter) (k : ikont) (t : abs2_term) (v1 v2 : val) : imonad iresult :=
-  let (b1, b2, t') := t in with_binder2 b1 b2 v1 v2 (self k t').
+Definition interpret_term2_aux (self : interpreter) (t : term2) (k : ikont) (v1 v2 : val) : imonad iresult :=
+  let (b1, b2, t') := t in imonad_local_env (fun env => with_binder b2 v2 (with_binder b1 v1 env)) (self t' k).
 
-Definition interpret_ret_term_with (self : interpreter) (k : ikont) (t : ret_term) (v : val) : imonad iresult :=
+Definition interpret_term1_aux_under (env : env) (self : interpreter) (t : term1) (k : ikont) (v : val) : imonad iresult :=
+  let (b, t') := t in imonad_under_env (with_binder b v env) (self t' k).
+
+Definition interpret_term2_aux_under (env : env) (self : interpreter) (t : term2) (k : ikont) (v1 v2 : val) : imonad iresult :=
+  let (b1, b2, t') := t in imonad_under_env (with_binder b2 v2 (with_binder b1 v1 env)) (self t' k).
+
+Definition interpret_ret_term_aux_under (env : env) (self : interpreter) (t : ret_term) (k : ikont) (v : val) : imonad iresult :=
   match t with
   | TRetNone => k v
-  | TRetSome b t' => with_binder b v (self k t')
+  | TRetSome b t' => imonad_under_env (with_binder b v env) (self t' k)
   end.
 
-Fixpoint interpret_exn_term_with (self : interpreter) (k : ikont) (t : exn_term) (exn : exn) : option (imonad iresult) :=
+Fixpoint interpret_exn_term_aux_under (env : env) (self : interpreter) (t : exn_term) (k : ikont) (exn : exn) : option (imonad iresult) :=
   match t with
   | TExnLast p t' =>
-      match match_exn p exn with
-      | Some f => Some (f (self k t'))
+      match match_exn p exn env with
+      | Some env' => Some (imonad_under_env env' (self t' k))
       | None => None
       end
   | TExnCons p t1 t2 =>
-      match match_exn p exn with
-      | Some f => Some (f (self k t1))
-      | None => interpret_exn_term_with self k t2 exn
+      match match_exn p exn env with
+      | Some env' => Some (imonad_under_env env' (self t1 k))
+      | None => interpret_exn_term_aux_under env self t2 k exn
       end
   end.
 
-Fixpoint interpret_eff_term_with (self : interpreter) (k : ikont) (t : eff_term) (eff : eff) (v : val) : option (imonad iresult) :=
+Fixpoint interpret_eff_term_aux_under (env : env) (self : interpreter) (t : eff_term) (k : ikont) (eff : eff) (v : val) : option (imonad iresult) :=
   match t with
   | TEffLast p b t' =>
-      match match_eff p b eff v with
-      | Some f => Some (f (self k t'))
+      match match_eff p b eff v env with
+      | Some env' => Some (imonad_under_env env' (self t' k))
       | None => None
       end
   | TEffCons p b t1 t2 =>
-      match match_eff p b eff v with
-      | Some f => Some (f (self k t1))
-      | None => interpret_eff_term_with self k t2 eff v
+      match match_eff p b eff v env with
+      | Some env' => Some (imonad_under_env env' (self t1 k))
+      | None => interpret_eff_term_aux_under env self t2 k eff v
       end
-  end.
-
-Definition interpret_kont_clo_with (self : interpreter) (k : ikont) (c : kont_clo) (v : val) : imonad iresult :=
-  match c with
-  | CKSeq env t => imonad_use_env env (self k t)
-  | CKLet env t => imonad_use_env env (interpret_abs_term_with self k t v)
   end.
 
 Definition unwind_try (self : interpreter) (c : try_clo) (k : ikont) (r : iresult) : imonad iresult :=
   match r with
-  | RVal v => k v
-  | RShift mk f tag => imonad_pure (RShift (MKTry mk c k) f tag)
-  | RControl mk f tag => imonad_pure (RControl (MKTry mk c k) f tag)
-  | RRaise exn =>
-      let (_, t) := c in
-      match interpret_exn_term_with self k t exn with
+  | IRVal v => k v
+  | IRShift mk f tag => imonad_pure (IRShift (MKTry mk c k) f tag)
+  | IRControl mk f tag => imonad_pure (IRControl (MKTry mk c k) f tag)
+  | IRRaise exn =>
+      let (env, t) := c in
+      match interpret_exn_term_aux_under env self t k exn with
       | Some m => m
       | None => imonad_pure r
       end
-  | RPerform mk eff => imonad_pure (RPerform (MKTry mk c k) eff)
+  | IRPerform mk eff => imonad_pure (IRPerform (MKTry mk c k) eff)
   end.
-
-Definition unwind_try_clo (self : interpreter) (c : try_clo) (k : ikont) (r : iresult) : imonad iresult :=
-  let (env, _) := c in imonad_use_env env (unwind_try self c k r).
 
 Definition unwind_handle (self : interpreter) (c : handle_clo) (k : ikont) (r : iresult) : imonad iresult :=
   match r with
-  | RVal v => let (_, t, _) := c in interpret_ret_term_with self k t v
-  | RShift mk f tag => imonad_pure (RShift (MKHandle mk c k) f tag)
-  | RControl mk f tag => imonad_pure (RControl (MKHandle mk c k) f tag)
-  | RRaise _ => imonad_pure r
-  | RPerform mk eff =>
-      let (_, _, t) := c in
-      match interpret_eff_term_with self k t eff (VMKHandle mk c) with
+  | IRVal v => let (env, t, _) := c in interpret_ret_term_aux_under env self t k v
+  | IRShift mk f tag => imonad_pure (IRShift (MKHandle mk c k) f tag)
+  | IRControl mk f tag => imonad_pure (IRControl (MKHandle mk c k) f tag)
+  | IRRaise _ => imonad_pure r
+  | IRPerform mk eff =>
+      let (env, _, t) := c in
+      match interpret_eff_term_aux_under env self t k eff (VMKHandle mk c) with
       | Some m => m
-      | None => imonad_pure (RPerform (MKHandle mk c k) eff)
+      | None => imonad_pure (IRPerform (MKHandle mk c k) eff)
       end
   end.
-
-Definition unwind_handle_clo (self : interpreter) (c : handle_clo) (k : ikont) (r : iresult) : imonad iresult :=
-  let (env, _, _) := c in imonad_use_env env (unwind_handle self c k r).
 
 Definition unwind_shallow_handle (self : interpreter) (c : shallow_handle_clo) (k : ikont) (r : iresult) : imonad iresult :=
   match r with
-  | RVal v => let (_, t, _) := c in interpret_ret_term_with self k t v
-  | RShift mk f tag => imonad_pure (RShift (MKShallowHandle mk c k) f tag)
-  | RControl mk f tag => imonad_pure (RControl (MKShallowHandle mk c k) f tag)
-  | RRaise _ => imonad_pure r
-  | RPerform mk eff =>
-      let (_, _, t) := c in
-      match interpret_eff_term_with self k t eff (VMKPure mk) with
+  | IRVal v => let (env, t, _) := c in interpret_ret_term_aux_under env self t k v
+  | IRShift mk f tag => imonad_pure (IRShift (MKShallowHandle mk c k) f tag)
+  | IRControl mk f tag => imonad_pure (IRControl (MKShallowHandle mk c k) f tag)
+  | IRRaise _ => imonad_pure r
+  | IRPerform mk eff =>
+      let (env, _, t) := c in
+      match interpret_eff_term_aux_under env self t k eff (VMKPure mk) with
       | Some m => m
-      | None => imonad_pure (RPerform (MKShallowHandle mk c k) eff)
+      | None => imonad_pure (IRPerform (MKShallowHandle mk c k) eff)
       end
   end.
 
-Definition unwind_shallow_handle_clo (self : interpreter) (c : shallow_handle_clo) (k : ikont) (r : iresult) : imonad iresult :=
-  let (env, _, _) := c in imonad_use_env env (unwind_shallow_handle self c k r).
+Definition interpret_kont_clo_aux (self : interpreter) (c : kont_clo) (k : ikont) (v : val) : imonad iresult :=
+  match c with
+  | CKSeq env t => imonad_under_env env (self t k)
+  | CKLet env t => interpret_term1_aux_under env self t k v
+  end.
 
-Fixpoint interpret_kont_with (self : interpreter) (k : kont) (ks : list kont) (f : val -> imonad iresult) (v : val) : imonad iresult :=
+Fixpoint interpret_kont_aux (self : interpreter) (k : kont) (v : val) : imonad iresult :=
   match k with
-  | KNil => f v
-  | KCons c k' => interpret_kont_clo_with self (IKont k' ks (interpret_kont_with self k' ks f)) c v
+  | KNil => imonad_pure (IRVal v)
+  | KCons c k' => interpret_kont_clo_aux self c (IKont k' (interpret_kont_aux self k')) v
+  | KApp k1 k2 => interpret_kont_aux self (IKont k1 (interpret_kont_aux self k2)) v
   end.
 
-Definition refine_kont (self : interpreter) (k1 : kont) (k2 : ikont) : ikont :=
-  let (h, t, f) := k2 in
-  let k2 := h :: t in
-  IKont k1 k2 (interpret_kont_with self k1 k2 f).
+Fixpoint interpret_kont_aux_app (self : interpreter) (k1 : kont) (k2 : ikont) (v : val) : imonad iresult :=
+  match k1 with
+  | KNil => k2 v
+  | KCons c k1' => interpret_kont_clo_aux self c (IKont (KApp k1' k2) (interpret_kont_aux_app self k1' k2)) v
+  | KApp k11 k12 => interpret_kont_aux_app self k11 (IKont (KApp k12 k2) (interpret_kont_aux_app self k12 k2)) v
+  end.
 
-Definition ikont_nil : ikont := IKont KNil nil (fun v => imonad_pure (RVal v)).
+Definition refine_kont (self : interpreter) (k : kont) : ikont :=
+  IKont k (interpret_kont_aux self k).
 
-Fixpoint interpret_metakont_with (self : interpreter) (k : ikont) (mk : metakont) (v : val) : imonad iresult :=
+Definition refine_kont_app (self : interpreter) (k1 : kont) (k2 : ikont) : ikont :=
+  IKont (KApp k1 k2) (interpret_kont_aux_app self k1 k2).
+
+Fixpoint interpret_metakont_aux (self : interpreter) (mk : metakont) (v : val) : imonad iresult :=
   match mk with
-  | MKPure k' => refine_kont self k' k v
-  | MKReset mk' tag k' => interpret_metakont_with self ikont_nil mk' v >>= unwind_reset tag (refine_kont self k' k)
-  | MKPrompt mk' tag k' => interpret_metakont_with self ikont_nil mk' v >>= unwind_prompt tag (refine_kont self k' k)
-  | MKTry mk' c k' => interpret_metakont_with self ikont_nil mk' v >>= unwind_try_clo self c (refine_kont self k' k)
-  | MKHandle mk' c k' => interpret_metakont_with self ikont_nil mk' v >>= unwind_handle_clo self c (refine_kont self k' k)
-  | MKShallowHandle mk' c k' => interpret_metakont_with self ikont_nil mk' v >>= unwind_shallow_handle_clo self c (refine_kont self k' k)
+  | MKPure k => interpret_kont_aux self k v
+  | MKReset mk' tag k => interpret_metakont_aux self mk' v >>= unwind_reset tag (refine_kont self k)
+  | MKPrompt mk' tag k => interpret_metakont_aux self mk' v >>= unwind_prompt tag (refine_kont self k)
+  | MKTry mk' c k => interpret_metakont_aux self mk' v >>= unwind_try self c (refine_kont self k)
+  | MKHandle mk' c k => interpret_metakont_aux self mk' v >>= unwind_handle self c (refine_kont self k)
+  | MKShallowHandle mk' c k => interpret_metakont_aux self mk' v >>= unwind_shallow_handle self c (refine_kont self k)
   end.
 
-Definition refine_term (self : interpreter) (k : ikont) (t : term) (env : env) (_ : val) : imonad iresult :=
-  imonad_use_env env (self k t).
+Definition interpret_metakont_aux_app (self : interpreter) (mk : metakont) (k : ikont) (v : val) : imonad iresult :=
+  match mk with
+  | MKPure k' => interpret_kont_aux_app self k' k v
+  | MKReset mk' tag k' => interpret_metakont_aux self mk' v >>= unwind_reset tag (refine_kont_app self k' k)
+  | MKPrompt mk' tag k' => interpret_metakont_aux self mk' v >>= unwind_prompt tag (refine_kont_app self k' k)
+  | MKTry mk' c k' => interpret_metakont_aux self mk' v >>= unwind_try self c (refine_kont_app self k' k)
+  | MKHandle mk' c k' => interpret_metakont_aux self mk' v >>= unwind_handle self c (refine_kont_app self k' k)
+  | MKShallowHandle mk' c k' => interpret_metakont_aux self mk' v >>= unwind_shallow_handle self c (refine_kont_app self k' k)
+  end.
 
-Definition refine_abs_term (self : interpreter) (k : ikont) (t : abs_term) (env : env) (v : val) : imonad iresult :=
-  imonad_use_env env (interpret_abs_term_with self k t v).
-
-Definition app_LFun (self : interpreter) (k : ikont) (c : fun_clo) (v : val) : imonad iresult :=
-  let (env, t) := c in imonad_use_env env (interpret_abs_term_with self k t v).
-
-Definition app_LFix (self : interpreter) (k : ikont) (c : fix_clo) (u v : val) : imonad iresult :=
-  let (env, t) := c in imonad_use_env env (interpret_abs2_term_with self k t u v).
-
-Definition app_LMKPure (self : interpreter) (k : ikont) (mk : metakont) (v : val) : imonad iresult :=
-  interpret_metakont_with self k mk v.
-
-Definition app_LMKReset (self : interpreter) (k : ikont) (mk : metakont) (tag : tag) (v : val) : imonad iresult :=
-  interpret_metakont_with self ikont_nil mk v >>= unwind_reset tag k.
-
-Definition app_LMKHandle (self : interpreter) (k : ikont) (mk : metakont) (c : handle_clo) (v : val) : imonad iresult :=
-  interpret_metakont_with self ikont_nil mk v >>= unwind_handle_clo self c k.
-
-Definition interpret_term_aux (self' : interpreter) : ikont -> term -> imonad iresult :=
-  fix self k t :=
+Definition interpret_term_aux (self : interpreter) : term -> ikont -> imonad iresult :=
+  fix self' (t : term) (k : ikont) : imonad iresult :=
     match t with
     | TVal t' => interpret_val_term t' >>= k
     | TApp t1 t2 =>
@@ -319,76 +293,74 @@ Definition interpret_term_aux (self' : interpreter) : ikont -> term -> imonad ir
         l <- unwrap_vlambda u;
         v <- interpret_val_term t2;
         match l with
-        | LFun c => app_LFun self' k c v
-        | LFix c => app_LFix self' k c u v
-        | LMKPure mk => app_LMKPure self' k mk v
-        | LMKReset mk tag => app_LMKReset self' k mk tag v
-        | LMKHandle mk c => app_LMKHandle self' k mk c v
+        | LFun c => let (env, t) := c in interpret_term1_aux_under env self t k v
+        | LFix c => let (env, t) := c in interpret_term2_aux_under env self t k u v
+        | LMKPure mk => interpret_metakont_aux_app self mk k v
+        | LMKReset mk tag => interpret_metakont_aux self mk v >>= unwind_reset tag k
+        | LMKHandle mk c => interpret_metakont_aux self mk v >>= unwind_handle self c k
         end
     | TSeq t1 t2 =>
         env <- imonad_ask_env;
-        let (h, t, _) := k in
-        self (IKont (KCons (CKSeq env t2) h) t (refine_term self k t2 env)) t1
+        self' t1 (IKont (KCons (CKSeq env t2) k) (fun _ => imonad_under_env env (self' t2 k)))
     | TLet t1 t2 =>
         env <- imonad_ask_env;
-        let (h, t, _) := k in
-        self (IKont (KCons (CKLet env t2) k) t (refine_abs_term self k t2 env)) t1
+        self' t1 (IKont (KCons (CKLet env t2) k) (interpret_term1_aux_under env self' t2 k))
     | TIf t1 t2 t3 =>
         v <- interpret_val_term t1;
         b <- unwrap_vbool v;
-        if b then self k t2 else self k t3
+        if b then self' t2 k else self' t3 k
     | TSplit t1 t2 =>
         v <- interpret_val_term t1;
         p <- unwrap_vprod v;
-        let (v1, v2) := p in interpret_abs2_term_with self k t2 v1 v2
+        let (v1, v2) := p in interpret_term2_aux self' t2 k v1 v2
     | TCase t1 t2 t3 =>
         v <- interpret_val_term t1;
         s <- unwrap_vsum v;
         match s with
-        | inl v' => interpret_abs_term_with self k t2 v'
-        | inr v' => interpret_abs_term_with self k t3 v'
+        | inl v' => interpret_term1_aux self' t2 k v'
+        | inr v' => interpret_term1_aux self' t3 k v'
         end
-    | TShift tag t' => imonad_asks_env (fun env => RShift (MKPure k) (refine_abs_term self ikont_nil t' env) tag)
-    | TReset tag t' => self ikont_nil t' >>= unwind_reset tag k
-    | TControl tag t' => imonad_asks_env (fun env => RControl (MKPure k) (refine_abs_term self ikont_nil t' env) tag)
-    | TPrompt tag t' => self ikont_nil t' >>= unwind_prompt tag k
+    | TShift tag t' => imonad_asks_env (fun env => IRShift (MKPure k) (interpret_term1_aux_under env self' t' ikont_nil) tag)
+    | TReset tag t' => self' t' ikont_nil >>= unwind_reset tag k
+    | TControl tag t' => imonad_asks_env (fun env => IRControl (MKPure k) (interpret_term1_aux_under env self' t' ikont_nil) tag)
+    | TPrompt tag t' => self' t' ikont_nil >>= unwind_prompt tag k
     | TRaise t' =>
         v <- interpret_val_term t';
-        RRaise <$> unwrap_vexn v
+        IRRaise <$> unwrap_vexn v
     | TTry t1 t2 =>
-        r <- self ikont_nil t1;
+        r <- self' t1 ikont_nil;
         env <- imonad_ask_env;
-        unwind_try self (CTry env t2) k r
+        unwind_try self' (CTry env t2) k r
     | TPerform t' =>
         v <- interpret_val_term t';
-        RPerform (MKPure k) <$> unwrap_veff v
+        IRPerform (MKPure k) <$> unwrap_veff v
     | THandle t1 t2 t3 =>
-        r <- self ikont_nil t1;
+        r <- self' t1 ikont_nil;
         env <- imonad_ask_env;
-        unwind_handle self (CHandle env t2 t3) k r
+        unwind_handle self' (CHandle env t2 t3) k r
     | TShallowHandle t1 t2 t3 =>
-        r <- self ikont_nil t1;
+        r <- self' t1 ikont_nil;
         env <- imonad_ask_env;
-        unwind_shallow_handle self (CShallowHandle env t2 t3) k r
+        unwind_shallow_handle self' (CShallowHandle env t2 t3) k r
     end.
 
-Fixpoint interpret_term (fuel : nat) (k : ikont) (t : term) : imonad iresult :=
+Fixpoint interpret_term (fuel : nat) (t : term) (k : ikont) : imonad iresult :=
   match fuel with
   | O => imonad_throw_error Out_of_fuel
-  | S fuel' => interpret_term_aux (interpret_term fuel') k t
+  | S fuel' => interpret_term_aux (interpret_term fuel') t k
   end.
 
-Definition unwrap_RVal (r : iresult) : imonad val :=
+Definition unwrap_IRVal (r : iresult) : imonad val :=
   match r with
-  | RVal v => imonad_pure v
-  | RShift _ _ tag => imonad_throw_error (Undelimited_shift tag)
-  | RControl _ _ tag => imonad_throw_error (Undelimited_control tag)
-  | RRaise exn => imonad_throw_error (Unhandled_exception exn)
-  | RPerform _ eff => imonad_throw_error (Unhandled_effect eff)
+  | IRVal v => imonad_pure v
+  | IRShift _ _ tag => imonad_throw_error (Undelimited_shift tag)
+  | IRControl _ _ tag => imonad_throw_error (Undelimited_control tag)
+  | IRRaise exn => imonad_throw_error (Unhandled_exception exn)
+  | IRPerform _ eff => imonad_throw_error (Unhandled_effect eff)
   end.
 
 Definition run_term (fuel : nat) (t : term) : (ierror + val) * iheap :=
-  imonad_run (interpret_term fuel ikont_nil t >>= unwrap_RVal) EnvNil iheap_empty.
+  imonad_run (interpret_term fuel t ikont_nil >>= unwrap_IRVal) EnvNil iheap_empty.
 
 Definition eval_term (fuel : nat) (t : term) : ierror + val :=
   fst (run_term fuel t).
